disk-betree/MutableBucket.i.dfy
@@ -1,5 +1,6 @@
 include "../lib/tttree.i.dfy"
 include "KVList.i.dfy"
+include "KVListPartialFlush.i.dfy"
 include "Bounds.i.dfy"
 
 module MutableBucket {
